cosmetic tweaks

ironfleet/src/Dafny/Distributed/Protocol/Lock/PerformanceProof/EmptyPerformanceProof.i.dfy
@@ -7,37 +7,62 @@ import opened LockTimestampedDistributedSystem_i
     import opened TimestampedGLS_i
     import opened PerformanceProof__Definitions_i
     import opened Math__mod_auto_i
+
+
+/*****************************************************************************************
+*                                 Performance Predicates                                 *
+*****************************************************************************************/
+
+
 predicate SingleGLSPerformanceAssumption(tgls:TimestampedGLS_State)
 {
     // The only nodes that take steps are in the ring
     && (tgls.tls.t_environment.nextStep.LEnvStepHostIos? ==> tgls.tls.t_environment.nextStep.actor in tgls.tls.t_servers)
     // The size of the history/epochs never reaches UINT64_MAX
     && (|tgls.history| < 0xFFFF_FFFF_FFFF_FFFF)
-    // No timeouts
+    // No timeouts. This means that NodeAccept never takes the LIoOpTimeoutReceive branch
     && (var nextStep := tgls.tls.t_environment.nextStep; nextStep.LEnvStepHostIos? ==>
     (forall io :: io in nextStep.ios ==> !io.LIoOpTimeoutReceive?))
     // TODO: This should be part of the state machine definition, and not an assumption
     // The only nodes that can do NodeGrant() currently hold the lock
-    && (var nextStep := tgls.tls.t_environment.nextStep; nextStep.LEnvStepHostIos? ==> (nextStep.nodeStep == GrantStep <==> tgls.tls.t_servers[nextStep.actor].v.held == true))
+    && (var nextStep := tgls.tls.t_environment.nextStep; nextStep.LEnvStepHostIos? ==> (nextStep.nodeStep == GrantStep <==> tgls.tls.t_servers[nextStep.actor].v.held))
 }
+
+
 predicate GLSPerformanceAssumption(tglb:seq<TimestampedGLS_State>)
 {
-    forall tgls :: tgls in tglb ==> SingleGLSPerformanceAssumption(tgls)
+    forall tgls | tgls in tglb :: SingleGLSPerformanceAssumption(tgls)
 }
+
+
 predicate SingleGLSPerformanceGuarantee(gls:TimestampedGLS_State)
+    requires |gls.tls.config| > 1;
 {
-    |gls.tls.config| > 1 ==> 
-    (forall pkt :: pkt in gls.tls.t_environment.sentPackets &&
-        pkt.msg.v == Transfer(|gls.tls.config|) ==> TimeEq(pkt.msg.ts, PerfBoundLockInNetwork(|gls.tls.config|)))
+    forall pkt  
+        | && pkt in gls.tls.t_environment.sentPackets 
+          && pkt.msg.v == Transfer(|gls.tls.config|) 
+        :: TimeEq(pkt.msg.ts, PerfBoundLockInNetwork(|gls.tls.config|))
 }
+
+
 predicate GLSPerformanceGuarantee(tglb:seq<TimestampedGLS_State>)
 {
-    forall tgls :: tgls in tglb ==> SingleGLSPerformanceGuarantee(tgls)
+    forall tgls | tgls in tglb :: SingleGLSPerformanceGuarantee(tgls)
 }
+
+
+/*****************************************************************************************
+*                                 Performance Theorem                                    *
+*****************************************************************************************/
+
+
+/* Main Performance Theorem */
 lemma PerformanceGuaranteeHolds(config:Config, tglb:seq<TimestampedGLS_State>)
+    requires |config| > 1;
     requires ValidTimestampedGLSBehavior(tglb, config)
     requires GLSPerformanceAssumption(tglb)
     ensures GLSPerformanceGuarantee(tglb)
 {
+    assume false;
 }
 }
